\documentclass[11pt, letterpaper]{article}
\usepackage[margin=1.5cm]{geometry}
\pagestyle{plain}

\usepackage{amsmath, amsfonts, amssymb, amsthm}
\usepackage{bbm}
\usepackage[shortlabels]{enumitem}
\usepackage[makeroom]{cancel}
\usepackage{graphicx}
\usepackage{calrsfs}
\usepackage{xcolor}
\usepackage{array, booktabs, ragged2e}
\graphicspath{{./Images/}}

\newcommand{\bs}[1]{\boldsymbol{#1}}
\newcommand{\mbb}[1]{\mathbb{#1}}
\newcommand{\mc}[1]{\mathcal{#1}}
\newcommand{\ra}[1]{\renewcommand{\arraystretch}{#1}}

\title{\bf Stochastic Processes: Assignment V}
\author{\bf Connor Braun}
\date{}

\begin{document}
    \maketitle
    \noindent{\bf Problem 6} Consider the setup in problem 4. For any integer $n\geq 0$, denote $m_n(t)$ the expected number of lines in use at time $t$, given that $n$
    are in use at time $0$. Show that
    \[m_n(t)=ne^{-\mu t}+\frac{\lambda}{\mu}(1-e^{-\mu t}).\]
    {\bf Proof} Suppose that there are $n\in\mbb{N}$ people in the queue at time $t=0$. Define the random variable $N(t)$ to be the number of people in the queue at time $t$.
    We can be decompose $N(t)$
    \[N(t)=K(t)+L(t)\]
    where $K(t)$ is the number of the original $n$ individuals who remain in the queue at time $t$, and $L(t)$ is the number of individuals
    who arrived later and remain in the queue by time $t$.\\[10pt]
    With this setup, let $K_j$ be the random variable for the time that the $j$th person (of the original $n$) leaves the queue. Then,
    \[K(t)=\sum_{j=1}^n\mathbbm{1}_{\{K_j>t\}}\quad\Rightarrow\quad\mbb{E}[K(t)]=\sum_{j=1}^nP(K_j>t)=\sum_{j=1}^ne^{-\mu t}=ne^{-\mu t}\]
    where $P(K_j>t)=e^{-\mu t}$ is the survival function of the $j$th person when the duration of their call is exponentially distributed with rate parameter $\mu$. Now, to compute the desired expectation
    \[m_n(t)=\mbb{E}[N(t)]=\mbb{E}[K(t)]+\mbb{E}[L(t)]=ne^{-\mu t}+m_0(t)\]
    we need only determine $m_0(t)$. To do this, we use the law of iterated expectation, conditioning on the value of the first holding time $S_1$.
    \begin{align*}
        m_0(t)=\mbb{E}[L(t)]=\mbb{E}_{S_1}[\mbb{E}[L(t)|S_1<t]]\tag{5}
    \end{align*}
    where we condition on $S_1<t$ since otherwise $L(t)=0$ {\it w.p.} 1 so that these instances do not influence the expectation. However, provided $S_1<t$ is fixed, the inner expectation can be expressed
    \[\mbb{E}[L(t)|S_1<t]=\mbb{E}[\mathbbm{1}_{\{L_1>t-S_1\}}+L(t-S_1)|S_1<t]=P(L_1>t-S_1)+m_0(t-S_1)=e^{-\mu(t-S_1)}+m_0(t-S_1)\]
    having let $L_1$ be the random variable for the time at which the first person to arrive departs. Returning to (5) we can now compute the outer expectation. Since $S_1\sim\text{Exp}\;(\lambda)$, we have
    \begin{align*}
        m_0(t)=\mbb{E}_{S_1}[e^{-\mu(t-S_1)}+m_0(t-S_1)|S_1<t]&=\int_{0}^t\left(e^{-\mu(t-x)}+m_0(t-x)\right)\lambda e^{-\lambda x}dx\\
        &=\int_0^t\left(e^{-\mu y}+m_0(y)\right)\lambda e^{-\lambda(t-y)}dy\tag{substituting $y=t-x$}\\
        &=e^{-\lambda t}\int_0^t\left(e^{-\mu y}+m_0(y)\right)\lambda e^{\lambda y}dy.
    \end{align*}
    From here, we differentiate $m_0(t)$ to obtain a first order, linear ordinary differential equation:
    \begin{align*}
        m_0^\prime(t)&=-\lambda e^{-\lambda t}\int_0^t\left(e^{-\mu y}+m_0(y)\right)\lambda e^{\lambda y}dy+e^{-\lambda t} \frac{d}{dt}\int_0^t\left(e^{-\mu y}+m_0(y)\right)\lambda e^{\lambda y}dy\\
        &=-\lambda \int_0^t\left(e^{-\mu y}+m_0(y)\right)\lambda e^{-\lambda (t-y)}dy+\lambda e^{-\lambda t}e^{\lambda t}(e^{-\mu t}+m_0(t))\\
        &=-\lambda m_0(t)+\lambda e^{-\mu t}+\lambda m_0(t)\\
        &=\lambda e^{-\mu t}.
    \end{align*}
    Supplying the initial condition that $m_0(0)=0$, we see that the second term in the proposed solution
    \[m_n(t)=ne^{-\mu t}+\frac{\lambda}{\mu}(1-e^{-\mu t})\]
    is the unique solution to $m_0^\prime(t)=\lambda e^{-\mu t}$, $m_0(0)=0$, since
    \begin{align*}
        \frac{\lambda}{\mu}(1-e^{-\mu t})\bigg|_{t=0}=0\quad\text{and}\quad\frac{d}{dt}\frac{\lambda}{\mu}(1-e^{-\mu t})=\lambda e^{-\mu t}=m_0^\prime(t).
    \end{align*}
    With this, we get
    \[m_n(t)=\mbb{E}[N(t)]=\mbb{E}[K(t)]+\mbb{E}[L(t)]=ne^{-\mu t}+m_0(t)=ne^{-\mu t}+\frac{\lambda}{\mu}(1-e^{-\mu t})\]
    as desired.\hfill{$\qed$}\\[10pt]
\end{document}